DIRTY WIP: Model stack frames as bytes
Similarly to how we model the register file as a kind of memory block that
stores bytes (more precisely, memvals), add a Stack module that does the
same for the stack frame. The three kinds of stack slots (incoming,
outgoing, local) each have their separate memval map that stores the data.

The idea is to allow us to model spilling as copying of bytes from registers
to the stack and back. This is meant to preserve spilled values, even if
those values are in the subregisters of a spilled superregister. This cannot
be modeled as copying values directly, since the value of a superregister is
undefined if one of its subregisters holds a value.

FIXME: Many many admits.

backend/Locations.v
@@ -317,6 +317,119 @@ Module Loc.
 
 End Loc.
 
+(** * Representation of the stack frame *)
+
+(** The [Stack] module defines mappings from stack slots to values,
+  represented as a mapping from addresses to bytes. The stack frame is
+  represented as three distinct such mappings, one for each kind of slot; a
+  stack slot [S sl ofs q] is accessed in the mapping for its kind [sl] at an
+  address computed from its offset [ofs], using [q] to inform how many bytes to
+  access and how to encode/decode them. *)
+
+Module Stack.
+
+  Definition t := slot -> ZMap.t memval.
+
+  Definition init : t := fun _ => ZMap.init Undef.
+
+  (* A slot's address: The index of its first byte. Offsets are expressed in
+     terms of words, so we must scale them. *)
+  Definition addr (ofs: Z) : Z := ofs * 4.
+
+  (* The address one byte past the end of a slot with [ofs] and [q]. The next
+     nonoverlapping slot may start here. *)
+  Definition next_addr (ofs: Z) (q: quantity) : Z := addr ofs * AST.typesize (typ_of_quantity q).
+
+  Definition get_bytes sl ofs q (stack: t) : list memval :=
+    Mem.getN (Z.to_nat (AST.typesize (typ_of_quantity q))) (addr ofs) (stack sl).
+
+  Definition get sl ofs q (stack: t) : val :=
+    decode_val (chunk_of_type (typ_of_quantity q)) (get_bytes sl ofs q stack).
+
+  Definition set_bytes sl ofs (bytes: list memval) (stack: t) : t :=
+    fun slot =>
+      if slot_eq slot sl then
+        Mem.setN bytes (addr ofs) (stack sl)
+      else
+        stack slot.
+
+  Definition set sl ofs q (v: val) (stack: t) : t :=
+    set_bytes sl ofs (encode_val (chunk_of_type (typ_of_quantity q)) v) stack.
+
+  Lemma chunk_length:
+    forall ty v,
+    Z.to_nat (AST.typesize ty) = length (encode_val (chunk_of_type ty) v).
+  Proof.
+    intros. rewrite encode_val_length. destruct ty; auto.
+  Qed.
+
+  Lemma gss:
+    forall sl ofs q v stack,
+    get sl ofs q (set sl ofs q v stack) = Val.load_result (chunk_of_type (typ_of_quantity q)) v.
+  Proof.
+    intros. unfold get, set, get_bytes, set_bytes.
+    rewrite dec_eq_true. erewrite chunk_length. rewrite Mem.getN_setN_same.
+    erewrite <- decode_encode_val_similar; eauto.
+    eapply decode_encode_val_general.
+  Qed.
+
+  Lemma gso:
+    forall sl ofs q sl' ofs' q' v stack,
+    Loc.diff (S sl ofs q) (S sl' ofs' q') ->
+    get sl ofs q (set sl' ofs' q' v stack) = get sl ofs q stack.
+  Proof.
+    intros. unfold get, set, get_bytes, set_bytes.
+    destruct (slot_eq sl sl'); subst; auto.
+    rewrite Mem.getN_setN_outside; auto.
+    rewrite <- chunk_length, !Z2Nat.id.
+    destruct H as [FALSE|]. contradiction.
+    assert (Size: forall t, AST.typesize t = 4 * typesize t) by (intro t; destruct t; auto).
+    rewrite !Size. unfold addr. omega.
+    destruct q'; simpl; omega.
+    destruct q; simpl; omega.
+  Qed.
+
+  Lemma gu_overlap:
+    forall sl ofs q sl' ofs' q' v stack,
+    S sl ofs q <> S sl' ofs' q' ->
+    ~ Loc.diff (S sl ofs q) (S sl' ofs' q') ->
+    get sl ofs q (set sl' ofs' q' v stack) = Vundef.
+  Proof.
+    admit.
+  Admitted.
+
+  Lemma gss_bytes:
+    forall sl ofs q bs rf,
+    let sz := Z.to_nat (AST.typesize (typ_of_quantity q)) in
+    length bs = sz ->
+    get_bytes sl ofs q (set_bytes sl ofs bs rf) = firstn sz bs.
+  Proof.
+    intros. unfold get_bytes, set_bytes.
+    subst sz. rewrite <- H. rewrite dec_eq_true, Mem.getN_setN_same.
+    rewrite firstn_all; auto.
+  Qed.
+
+  Lemma gso_bytes:
+    forall sl ofs q sl' ofs' q' bs stack,
+    let sz := Z.to_nat (AST.typesize (typ_of_quantity q)) in
+    length bs = sz ->
+    Loc.diff (S sl ofs q) (S sl' ofs' q') ->
+    get_bytes sl' ofs' q' (set_bytes sl ofs bs stack) = get_bytes sl' ofs' q' stack.
+  Proof.
+    intros. unfold get_bytes, set_bytes.
+    destruct (slot_eq sl sl'); subst; auto.
+    rewrite dec_eq_true, Mem.getN_setN_outside; auto.
+    rewrite H. subst sz.
+    destruct H0 as [FALSE|]. contradiction.
+    assert (Size: forall t, AST.typesize t = 4 * typesize t) by (intro t; destruct t; auto).
+    rewrite !Size, !Z2Nat.id. unfold addr. omega.
+    destruct q; simpl; omega.
+    destruct q'; simpl; omega.
+    rewrite dec_eq_false; auto.
+  Qed.
+
+End Stack.
+
 (** * Mappings from locations to values *)
 
 (** The [Locmap] module defines mappings from locations to values,
@@ -327,17 +440,17 @@ Set Implicit Arguments.
 
 Module Locmap.
 
-  Definition t := (Regfile.t * (loc -> list memval))%type.
+  Definition t := (Regfile.t * Stack.t)%type.
 
   Definition chunk_of_loc (l: loc) : memory_chunk :=
     chunk_of_type (Loc.type l).
 
-  Definition init : t := (Regfile.init, fun (l: loc) => encode_val (chunk_of_loc l) Vundef).
+  Definition init : t := (Regfile.init, Stack.init).
 
   Definition get (l: loc) (m: t) : val :=
     match l, m with
     | R r, (rf, stack) => Regfile.get r rf
-    | S _ _ _, (rf, stack) => decode_val (chunk_of_loc l) (stack l)
+    | S sl ofs ty, (rf, stack) => Stack.get sl ofs ty stack
     end.
 
   (* Auxiliary for some places where a function of type [loc -> val] is expected. *)
@@ -356,28 +469,18 @@ Module Locmap.
       abstract stack slots are mapped to concrete memory locations
       in the [Stacking] phase.  Hence, values stored in stack slots
       are normalized according to the type of the slot. *)
+  (** FIXME: The above comment is now out of date. *)
 
   Definition set (l: loc) (v: val) (m: t) : t :=
     match l, m with
     | R r, (rf, stack) => (Regfile.set r v rf, stack)
-    | S _ _ _, (rf, stack) => (rf,
-      fun (p: loc) =>
-        if Loc.eq l p then
-          encode_val (chunk_of_loc l) v
-        else if Loc.diff_dec l p then
-          stack p
-        else
-          encode_val (chunk_of_loc l) Vundef)
+    | S sl ofs ty, (rf, stack) => (rf, Stack.set sl ofs ty v stack)
     end.
 
   Lemma gss: forall l v m,
     get l (set l v m) = Val.load_result (chunk_of_type (Loc.type l)) v.
   Proof.
-    intros.
-    destruct l, m. apply Regfile.gss.
-    unfold get, set. rewrite dec_eq_true.
-    erewrite <- decode_encode_val_similar; eauto.
-    eapply decode_encode_val_general.
+    intros. destruct l, m. apply Regfile.gss. apply Stack.gss.
   Qed.
 
   Lemma gss_reg: forall r v m, Val.has_type v (mreg_type r) -> get (R r) (set (R r) v m) = v.
@@ -395,11 +498,7 @@ Module Locmap.
     intros.
     destruct l, m.
     destruct p; simpl in H; auto. apply Regfile.gso; auto using Registerfile.diff_sym.
-    unfold get, set. destruct (Loc.eq (S sl pos q) p).
-    subst p. elim (Loc.same_not_diff _ H).
-    destruct (Loc.diff_dec (S sl pos q) p).
-    auto.
-    contradiction.
+    destruct p. simpl in H; auto. apply Stack.gso; auto using Loc.diff_sym.
   Qed.
 
   Fixpoint undef (ll: list loc) (m: t) {struct ll} : t :=
@@ -424,19 +523,25 @@ Module Locmap.
       destruct a, l, m; simpl in n.
       simpl. rewrite Regfile.gu_overlap; auto.
       apply mreg_overlap_sym. apply not_same_not_diff_overlap; congruence.
-      auto. auto. unfold get, set. rewrite dec_eq_false; auto.
-      destruct (Loc.diff_dec (S sl pos q) (S sl0 pos0 q0)). auto. apply decode_encode_undef. }
+      auto. auto.
+      fold (Loc.diff (S sl pos q) (S sl0 pos0 q0)) in n.
+      unfold get, set. rewrite Stack.gu_overlap; auto using Loc.diff_sym. }
     induction ll; simpl; intros. contradiction.
     destruct H. apply P. subst a. apply gss_typed. exact I.
     auto.
   Qed.
 
   Lemma gu_overlap:
-    forall r s v m,
-    mreg_overlap r s ->
-    get (R r) (set (R s) v m) = Vundef.
+    forall l l' v m,
+    l <> l' ->
+    ~ Loc.diff l l' ->
+    get l (set l' v m) = Vundef.
   Proof.
-    intros; simpl. destruct m. auto using Regfile.gu_overlap.
+    intros. destruct l, l'; simpl in H0; try contradiction.
+    destruct m; simpl.
+    apply Regfile.gu_overlap. apply not_same_not_diff_overlap; congruence.
+    destruct m; simpl.
+    apply Stack.gu_overlap; auto.
   Qed.
 
   Definition getpair (p: rpair loc) (m: t) : val :=
@@ -477,6 +582,49 @@ Module Locmap.
     | BR_splitlong hi lo =>
         set (R lo) (Val.loword v) (set (R hi) (Val.hiword v) m)
     end.
+
+  (* Location access as raw bytes. This is used for spilling: When spilling a
+    superregister, we must store its bytes to the stack and later restore them.
+    This cannot be expressed in terms of values because the superregister has an
+    undefined value if any of its subregisters has a defined value and vice
+    versa. In either case, values are restored correctly, since restoring a
+    concrete list of bytes restores whatever interpretation it had in terms of
+    values. *)
+
+  Definition get_bytes (l: loc) (m: t) : list memval :=
+    match l, m with
+    | R r, (rf, stack) => Regfile.get_bytes r rf
+    | S sl ofs ty, (rf, stack) => Stack.get_bytes sl ofs ty stack
+    end.
+
+  Definition set_bytes (l: loc) (bs: list memval) (m: t) : t :=
+    match l, m with
+    | R r, (rf, stack) => (Regfile.set_bytes r bs rf, stack)
+    | S sl ofs ty, (rf, stack) => (rf, Stack.set_bytes sl ofs bs stack)
+    end.
+
+  Lemma gss_bytes: forall l bs m,
+    let sz := Z.to_nat (AST.typesize (Loc.type l)) in
+    length bs = sz ->
+    get_bytes l (set_bytes l bs m) = firstn sz bs.
+  Proof.
+    intros. destruct l, m.
+    apply Regfile.gss_bytes; auto.
+    apply Stack.gss_bytes; auto.
+  Qed.
+
+  Lemma gso_bytes: forall l bs m p,
+    let sz := Z.to_nat (AST.typesize (Loc.type l)) in
+    length bs = sz ->
+    Loc.diff l p ->
+    get_bytes p (set_bytes l bs m) = get_bytes p m.
+  Proof.
+    intros. destruct l, m, p.
+    apply Regfile.gso_bytes; auto.
+    simpl; auto.
+    simpl; auto.
+    eapply Stack.gso_bytes; eauto.
+  Qed.
 
 End Locmap.
 
